Demonstrate how to simplify blake2 streaming

code/streaming/Hacl.Streaming.Blake2.fst
@@ -7,13 +7,9 @@ module S = FStar.Seq
 module U32 = FStar.UInt32
 module U64 = FStar.UInt64
 module U128 = FStar.UInt128
-module Case = FStar.Int.Cast.Full
 module F = Hacl.Streaming.Functor
 module I = Hacl.Streaming.Interface
 module ST = FStar.HyperStack.ST
-
-module Agile = Spec.Agile.Hash
-module Hash = Spec.Hash.Definitions
 
 open LowStar.BufferOps
 open FStar.Mul
@@ -21,7 +17,7 @@ open FStar.Mul
 module Loops = Lib.LoopCombinators
 
 /// Opening a bunch of modules for Blake2
-/// =======================================
+/// =====================================
 
 inline_for_extraction noextract
 let uint8 = Lib.IntTypes.uint8
@@ -33,17 +29,13 @@ module Spec = Spec.Blake2
 open Hacl.Impl.Blake2.Core
 module Core = Hacl.Impl.Blake2.Core
 open Hacl.Impl.Blake2.Generic
-module Incr = Spec.Hash.Incremental
 module Blake2s32 = Hacl.Blake2s_32
 module Blake2b32 = Hacl.Blake2b_32
 
 /// An instance of the stateful type class for blake2
-/// =========================================================
+/// =================================================
 
 #set-options "--max_fuel 0 --max_ifuel 0 --z3rlimit 200"
-
-inline_for_extraction noextract
-let to_hash_alg (a : Spec.alg) = Hash.to_hash_alg a
 
 inline_for_extraction noextract
 let index = unit
@@ -59,12 +51,11 @@ inline_for_extraction noextract
 let s (a : alg) (m : m_spec) = state_p a m & state_p a m
 
 inline_for_extraction noextract
-let extra_state_zero_element a : Hash.extra_state (to_hash_alg a) =
-  Hash.nat_to_extra_state (to_hash_alg a) 0
+let t (a : alg) = Spec.state a
 
-inline_for_extraction noextract
-let t (a : alg) = Hash.words_state' (to_hash_alg a)
-
+(* In the internal state, we keep wv, the working vector. It's essentially
+temporary scratch space that the Blake2 implementation expects to receive. (Why
+is the implementation not performing its own stack allocations? Don't know!) *)
 inline_for_extraction noextract
 let get_wv (#a : alg) (#m : m_spec) (s : s a m) : Tot (state_p a m) =
   match s with wv, _ -> wv
@@ -73,6 +64,8 @@ inline_for_extraction noextract
 let get_state_p (#a : alg) (#m : m_spec) (s : s a m) : Tot (state_p a m) =
   match s with _, p -> p
 
+(* But the working vector is not reflected in the state at all -- it doesn't
+have meaningful specification contents. *)
 inline_for_extraction noextract
 let state_v (#a : alg) (#m : m_spec) (h : HS.mem) (s : s a m) : GTot (Spec.state a) =
   Core.state_v h (get_state_p s)
@@ -136,8 +129,9 @@ let stateful_blake2 (a : alg) (m : m_spec) : I.stateful unit =
       B.blit (state_to_lbuffer src_b) 0ul (state_to_lbuffer dst_b) 0ul
              U32.(4ul *^ row_len a m))
 
-// Rk.: this is not necessary anymore, as well as stateful_key_t and stateful_key.
-// We keep those definitions here, though, because they may be useful in the future.
+/// Stateful key
+/// ============
+
 inline_for_extraction noextract
 let key_size_ty (a : alg) = key_size:nat{0 <= key_size /\ key_size <= Spec.max_key a}
 
@@ -222,21 +216,19 @@ let stateful_key_to_buffer (#a : alg) (#no_key : bool) (#key_size : key_size_t a
   b:B.buffer uint8 { B.length b = U32.v key_size } =
   if no_key then B.null #uint8 else key
 
-inline_for_extraction noextract  
+inline_for_extraction noextract
 let k = stateful_key
 
-/// The functor currently limits the size of the data, so we can't go as far as blake2b can go
-#push-options "--z3cliopt smt.arith.nl=false"
-noextract
-let max_total_hash_length (a : alg) :
-  n:nat{n `Spec.Hash.Definitions.less_than_max_input_length` (to_hash_alg a)} =
-  assert_norm(
-    Spec.max_limb Spec.Blake2S <= Some?.v(Spec.Hash.Definitions.max_input_length (to_hash_alg a)));
-  Spec.max_limb Spec.Blake2S
-#pop-options
+/// Actual functor instantiation
+/// ============================
+
+/// Small helpers
+/// -------------
 
 noextract
-let max_input_length (a : alg) : nat = max_total_hash_length a
+let max_input_length (a : alg) : n:nat { n <= Spec.max_limb a } =
+  assert_norm (pow2 64 < pow2 128);
+  pow2 64 - 1
 
 noextract inline_for_extraction
 let max_input_len (a: alg): (x:U64.t { U64.v x == max_input_length a }) = 0xffffffffffffffffUL
@@ -253,7 +245,8 @@ let output_size (a : alg) : nat = Spec.max_output a
 inline_for_extraction noextract
 let output_len (a : alg) = U32.uint_to_t (output_size a)
 
-/// Same function as above but with low-level types
+/// From the functor-provided previous length (uint64, public) to a suitable
+/// type for Blake2 (secret uint64/uint128)
 inline_for_extraction noextract
 let blake2_prevlen (a : alg)
                    (prevlen : U64.t{ U64.v prevlen <= max_input_length a}) :
@@ -266,64 +259,58 @@ let blake2_prevlen (a : alg)
     [@inline_let] let x : uint64 = to_u64 #U64 #PUB prevlen in
     Lib.IntTypes.cast U128 SEC x
 
+/// Specs
+/// -----
+
 noextract
-let init_s (a : alg) () :
+let init_s (a : alg) :
   Tot (t a) =
   Spec.blake2_init_hash a 0 (output_size a)
 
 noextract
-let update_multi_s (#a : alg) () (acc : t a)
+let update_multi_s (#a : alg) (acc : t a)
                    (prevlen : nat{prevlen % Spec.size_block a = 0})
                    (input : Seq.seq uint8{ prevlen + S.length input <= max_input_length a /\
                                            S.length input % Spec.size_block a = 0 }) :
-  Tot (t a) =
-  let es = Hash.nat_to_extra_state (to_hash_alg a) prevlen in
-  let s = (acc, es) in
-  fst (Agile.update_multi (to_hash_alg a) s input)
+  Tot (t a)
+=
+  let nb = S.length input / U32.v (block_len a) in
+  Lib.LoopCombinators.repeati nb (Spec.blake2_update1 a prevlen input) acc
 
 noextract
-let update_last_s (#a : alg) () (acc : t a)
+let update_last_s (#a : alg) (acc : t a)
                   (prevlen : nat{prevlen % Spec.size_block a = 0})
                   (input : Seq.seq uint8{ S.length input + prevlen <= max_input_length a /\
                                           S.length input <= Spec.size_block a }) :
   Tot (t a) =
-  let es = Hash.nat_to_extra_state (to_hash_alg a) prevlen in
-  let s = (acc, es) in
-  fst (Spec.Hash.Incremental.update_last (to_hash_alg a) s prevlen input)
+  Spec.blake2_update_last a prevlen (S.length input) input acc
 
 noextract
-let finish_s (#a : alg) () (acc : t a) :
+let finish_s (#a : alg) (acc : t a) :
   output : S.seq uint8 { S.length output = U32.v (output_len a) } =
-  (* The extra state is actually not used, so we initialize it to a dummy value *)
-  let s = (acc, Hash.nat_to_extra_state (to_hash_alg a) 0) in
-  Spec.Hash.PadFinish.finish (to_hash_alg a) s
+  Spec.blake2_finish a acc (U32.v (output_len a))
 
 noextract
-let spec_s (a : alg) () (_key : unit)
-           (input : S.seq uint8{S.length input <= max_input_length a}) = 
+let spec_s (a : alg) (_key : unit)
+           (input : S.seq uint8{S.length input <= max_input_length a}) =
   Spec.blake2 a input 0 Seq.empty (output_size a)
 
 /// Interlude for spec proofs
-/// =====================================
-noextract
+/// -------------------------
+
 val update_multi_zero:
   #a : alg ->
-  i:index ->
   acc:t a ->
   prevlen:nat{prevlen % Spec.size_block a = 0} ->
   Lemma
   (requires (prevlen <= max_input_length a))
-  (ensures (update_multi_s #a i acc prevlen S.empty == acc))
+  (ensures (update_multi_s #a acc prevlen S.empty == acc))
 
-let update_multi_zero #a () acc prevlen =
-  let es = Hash.nat_to_extra_state (to_hash_alg a) prevlen in
-  let s = (acc, es) in
-  Spec.Hash.Lemmas.update_multi_zero (to_hash_alg a) s
+let update_multi_zero #a acc prevlen =
+  Lib.LoopCombinators.eq_repeati0 (0 / U32.v (block_len a)) (Spec.blake2_update1 a prevlen S.empty) acc
 
-noextract
 val update_multi_associative:
   #a : alg ->
-  i:index ->
   acc: t a ->
   prevlen1:nat ->
   prevlen2:nat ->
@@ -340,331 +327,68 @@ val update_multi_associative:
     let input = S.append input1 input2 in
     S.length input % Spec.size_block a = 0 /\
     prevlen2 % Spec.size_block a = 0 /\
-    update_multi_s i (update_multi_s i acc prevlen1 input1) prevlen2 input2 ==
-      update_multi_s i acc prevlen1 input))
+    update_multi_s (update_multi_s acc prevlen1 input1) prevlen2 input2 ==
+      update_multi_s acc prevlen1 input))
 
-let update_multi_associative #a () acc prevlen1 prevlen2 input1 input2 =
-  let es = Hash.nat_to_extra_state (to_hash_alg a) prevlen1 in
-  let s = (acc, es) in
-  Spec.Hash.Lemmas.update_multi_associative (to_hash_alg a) s input1 input2;
-  Spec.Hash.Incremental.Lemmas.update_multi_extra_state_eq (to_hash_alg a) s input1;
-  Spec.Hash.Lemmas.extra_state_add_nat_bound_lem2 #(to_hash_alg a) es (S.length input1)
- 
+let update_multi_associative #a acc prevlen1 prevlen2 input1 input2 =
+  let input = S.append input1 input2 in
+  let nb = S.length input / U32.v (block_len a) in
+  let f = Spec.blake2_update1 a prevlen1 input in
+  (* calc (==) {
+    update_multi_s () acc prevlen1 input;
+  (==) { }
+    Lib.LoopCombinators.repeati nb (Spec.blake2_update1 a prevlen1 input) acc;
+  (==) { }
+    Lib.LoopCombinators.repeati nb f acc;
+  (==) { Lib.Sequence.Lemmas.repeati_extensionality }
+    Lib.LoopCombinators.repeati nb (Lib.Sequence.repeat_blocks_f (U32.v (block_len a)) input f nb) acc;
+  (==) { Lib.Sequence.lemma_repeat_blocks_multi ... }
+    Lib.LoopCombinators.repeat_blocks_multi ...
+  (==) { Lib.Sequence.Lemmas.repeat_blocks_multi_split ... }
+    Lib.LoopCombinators.(repeat_blocks_multi ... (repeat_blocks_multi ...))
+  ... inverse direction ...
+  }; *)
+  admit ()
+
 /// A helper function: the hash incremental function defined with the functions
 /// locally defined (with a signature adapted to the functor).
 noextract
 val blake2_hash_incremental_s :
   a : alg ->
-  i:index ->
   input:S.seq uint8 { S.length input <= max_input_length a} ->
   output:S.seq uint8 { S.length output = output_size a }
 
-noextract
-let size_block_props (a : Spec.alg) :
-  Lemma(
-    Spec.size_block a = Spec.Hash.Definitions.block_length (to_hash_alg a) /\
-    Spec.size_block a > 0) = ()
-
 #push-options "--z3cliopt smt.arith.nl=false"
-let blake2_hash_incremental_s a i input =
-  (**) size_block_props a;
-  (**) Math.Lemmas.modulo_lemma 0 (Spec.size_block a);
-  let bs, l = Spec.Hash.Incremental.split_blocks (to_hash_alg a) input in
-  let acc1 = init_s a i in
-  let acc2 = update_multi_s #a i acc1 0 bs in
-  let acc3 = update_last_s #a i acc2 (S.length bs) l in
-  let acc4 = finish_s #a i acc3 in
+let blake2_hash_incremental_s a input =
+  (**) Math.Lemmas.modulo_lemma 0 (U32.v (block_len a));
+  let bs, l = Lib.UpdateMulti.split_at_last_lazy (U32.v (block_len a)) input in
+  let acc1 = init_s a in
+  let acc2 = update_multi_s #a acc1 0 bs in
+  let acc3 = update_last_s #a acc2 (S.length bs) l in
+  let acc4 = finish_s #a acc3 in
   acc4
 #pop-options
 
-/// The following helper lemmas prove that the blake2 specification functions defined above
-/// with a signature adapted to the functor give the same result, if properly called,
-/// as the original hash incremental functions.
-noextract
-val blake2_hash_incremental_s_is_hash_incremental :
+val spec_is_incremental :
   a : alg ->
-  i:index ->
   input:S.seq uint8 { S.length input <= max_input_length a } ->
   Lemma(
-    blake2_hash_incremental_s a i input ==
-      Spec.Hash.Incremental.hash_incremental (to_hash_alg a) input)
+    blake2_hash_incremental_s a input ==
+      Spec.blake2 a input 0 S.empty (output_size a))
 
-noextract
-let init_s_blake2_init_eq
-  (a : alg)
-  (i:index) :
-  Lemma(
-    (init_s a i,
-     Hash.nat_to_extra_state (to_hash_alg a) 0) ==
-      Spec.Agile.Hash.init (to_hash_alg a)) =
-  Spec.Hash.Lemmas.reveal_init_blake2 a
+let spec_is_incremental a input =
+  let n_blocks, l_last = Spec.split a (S.length input) in
+  let blocks, last = Lib.UpdateMulti.split_at_last_lazy (U32.v (block_len a)) input in
+  let s = init_s a in
+  let s1 = Lib.LoopCombinators.repeati n_blocks (Spec.blake2_update1 a 0 input) s in
+  let s2 = Lib.LoopCombinators.repeati n_blocks (Spec.blake2_update1 a 0 blocks) s in
+  Lib.Sequence.Lemmas.repeati_extensionality n_blocks (Spec.blake2_update1 a 0 input)
+    (Spec.blake2_update1 a 0 blocks) s;
+  S.lemma_eq_intro (S.slice input (S.length input - l_last) (S.length input)) last;
+  S.lemma_eq_intro (S.slice last (S.length last - l_last) (S.length last)) last
 
-#push-options "--z3cliopt smt.arith.nl=false"
-let blake2_hash_incremental_s_is_hash_incremental a i input =
-  size_block_props a;
-  Math.Lemmas.modulo_lemma 0 (Spec.size_block a);
-  let bs, l = Spec.Hash.Incremental.split_blocks (to_hash_alg a) input in
-  let acc1 = init_s a i in
-  let acc2 = update_multi_s i acc1 0 bs in
-  let acc3 = update_last_s i acc2 (S.length bs) l in
-  let acc4 = finish_s #a i acc3 in
-  assert(acc4 == blake2_hash_incremental_s a i input); (* sanity check *)
-  let s1 = Spec.Agile.Hash.init (to_hash_alg a) in
-  let s2 = Agile.update_multi (to_hash_alg a) s1 bs in
-  let prevlen = S.length bs in (* dummy value: this variable is actually not used *)
-  let s3 = Spec.Hash.Incremental.update_last (to_hash_alg a) s2 prevlen l in
-  let s4 = Spec.Hash.PadFinish.finish (to_hash_alg a) s3 in
-  let s4' = Spec.Hash.Incremental.hash_incremental (to_hash_alg a) input in
-  assert(s4 == s4'); (* sanity check *)
-  (* The proof *)
-  (* 1 *)
-  let es1 = Hash.nat_to_extra_state (to_hash_alg a) 0 in
-  let s1' = (acc1, es1) in
-  init_s_blake2_init_eq a i;
-  assert(s1' == s1);
-  (* 2 *)
-  Spec.Hash.Incremental.Lemmas.update_multi_extra_state_eq (to_hash_alg a) s1 bs;
-  Spec.Hash.Lemmas.extra_state_v_of_nat (to_hash_alg a) 0;
-  assert(Hash.extra_state_v es1 + S.length bs <= Hash.max_extra_state (to_hash_alg a));
-  Spec.Hash.Lemmas.extra_state_add_nat_bound_lem2 #(to_hash_alg a) es1 (S.length bs);
-  let es2 = Hash.nat_to_extra_state (to_hash_alg a) (S.length bs) in
-  let s2' = (acc2, es2) in
-  assert(s2' == s2);
-  (* 3 *)
-  let es3 = Hash.nat_to_extra_state (to_hash_alg a) 0 in
-  let s3' = (acc3, es3) in
-  assert(s3' == s3);
-  (* 4 *)
-  assert(acc4 == s4)
-#pop-options
-
-#push-options "--z3cliopt smt.arith.nl=false"
-noextract
-val spec_is_incremental:
-  a : alg ->
-  i:index ->
-  input:S.seq uint8 { S.length input <= max_input_length a } ->
-  Lemma (
-    (**) size_block_props a;
-    (**) Math.Lemmas.modulo_lemma 0 (Spec.size_block a);
-    let bs, l = Lib.UpdateMulti.split_at_last_lazy (U32.v (block_len a)) input in
-    let hash0 = init_s a i in
-    let hash1 = update_multi_s i hash0 0 bs in
-    let hash2 = update_last_s i hash1 (S.length bs) l in
-    let hash3 = finish_s #a i hash2 in
-    hash3 `S.equal` spec_s a i () input)
-#pop-options
-
-#push-options "--z3cliopt smt.arith.nl=false"
-let spec_is_incremental a i input =
-  blake2_hash_incremental_s_is_hash_incremental a i input;
-  (**) size_block_props a;
-  Spec.Blake2.Incremental.blake2_is_hash_incremental (to_hash_alg a) input
-#pop-options
-
-noextract
-val update_multi_eq :
-  #a : alg ->
-  nb : nat ->
-  acc : t a ->
-  prevlen : nat {prevlen % Spec.size_block a = 0 } ->
-  blocks : S.seq uint8 ->
-  Lemma
-    (requires (
-      prevlen + S.length blocks <= max_input_length a /\
-      prevlen + S.length blocks <= Hash.max_extra_state (to_hash_alg a) /\
-      S.length blocks = Hash.block_length (to_hash_alg a) * nb))
-    (ensures (
-      update_multi_s () acc prevlen blocks ==
-        Loops.repeati #(Hash.words_state' (to_hash_alg a)) nb
-                       (Spec.blake2_update1 a prevlen blocks) acc))
-
-let update_multi_eq #a nb acc prevlen blocks =
-  let blocks', _ = Seq.split blocks (nb * Hash.block_length (to_hash_alg a)) in
-  assert(blocks' `Seq.equal` blocks);
-  let es = Hash.nat_to_extra_state (to_hash_alg a) prevlen in
-  Spec.Blake2.Incremental.repeati_blake2_update1_is_update_multi (to_hash_alg a)
-                                                               nb prevlen
-                                                               blocks acc;
-  Spec.Hash.Lemmas.extra_state_add_nat_bound_lem1 #(to_hash_alg a) es (S.length blocks);
-  assert(
-    Hash.nat_to_extra_state (to_hash_alg a) (prevlen + S.length blocks) ==
-    Hash.extra_state_add_nat #(to_hash_alg a) es (S.length blocks))
-
-noextract
-val update_last_eq :
-  #a : alg ->
-  prevlen : nat{prevlen % Hash.block_length (to_hash_alg a) = 0} ->
-  last : S.seq uint8 {S.length last <= Hash.block_length (to_hash_alg a) /\
-                      prevlen + S.length last <= max_input_length a} ->
-  acc : t a ->
-  Lemma
-  (ensures (
-    Spec.blake2_update_last a prevlen (S.length last) last acc ==
-      update_last_s () acc prevlen last))
-
-/// TODO: make stable - this proof was checked with quake and sometimes (very rarely) loops
-let update_last_eq #a prevlen last acc =
-  (* Checking how to unfold the ``update_last_s`` definition *)
-  let es = Hash.nat_to_extra_state (to_hash_alg a) prevlen in
-  let s = acc, es in
-  let s' = Spec.Hash.Incremental.update_last_blake (to_hash_alg a) s prevlen last in
-  (* TODO: SH: if accf is defined before s', the proof loops at the definition of s' *)
-  let accf = update_last_s () acc prevlen last in
-  assert(accf == fst s');
-  (* Make sure the blocks decomposition is what we expect *)
-  let blocks, last_block, rem = Spec.Hash.Incremental.last_split_blake (to_hash_alg a) last in
-  assert(blocks `S.equal` S.empty);
-  assert(rem = S.length last);
-  assert(last_block == Spec.get_last_padded_block a last (S.length last));
-  (* Prove that the last call to ``update_multi`` does nothing (there is no call to
-   * ``update_multi`` in ``blake2_update_last``) *)
-  let s2 = Spec.Agile.Hash.update_multi (to_hash_alg a) s blocks in
-  Spec.Hash.Lemmas.update_multi_zero (to_hash_alg a) s;
-  assert(s2 == s);
-  (* Prove that the extra state update computes the same total length as in ``blake2_update_last`` *)
-  Spec.Hash.Lemmas.extra_state_add_nat_bound_lem1 #(to_hash_alg a) es (S.length last);
-  assert(Hash.extra_state_v (Hash.extra_state_add_nat es (S.length last)) ==
-         Hash.extra_state_v es + S.length last)
-
-/// TODO: duplicate with Spec.Hash.Incremental.fst - MOVE
-/// Equality between the state types defined by blake2s and the generic hash.
-/// The equality is not trivial because of subtleties linked to the way types are
-/// encoded for Z3.
-noextract
-val state_types_equalities : (a : alg) ->
-  Lemma(Spec.Blake2.state a == Hash.words_state' (to_hash_alg a))
-
-let state_types_equalities a =
-  let open Lib.Sequence in
-  let open Lib.IntTypes in
-  (* Because of the necessity to be able to normalize, we basically do
-   * the same proof twice. TODO: find a better way *)
-  match a with
-  | Spec.Blake2S ->
-    let a = Spec.Blake2S in (* small trick to get a proper normalization *)
-    let row = Spec.row a in
-    assert(Spec.state a == lseq row 4);
-    assert_norm(Hash.words_state' (to_hash_alg a) == m:Seq.seq row {Seq.length m = 4});
-    assert_norm(lseq row 4 == m:Seq.seq row {Seq.length m == 4});
-    assert(lseq row 4 == m:Seq.seq row {Seq.length m = 4})
-  | Spec.Blake2B ->
-    let a = Spec.Blake2B in
-    let row = Spec.row a in
-    assert(Spec.state a == lseq row 4);
-    assert_norm(Hash.words_state' (to_hash_alg a) == m:Seq.seq row {Seq.length m = 4});
-    assert_norm(lseq row 4 == m:Seq.seq row {Seq.length m == 4});
-    assert(lseq row 4 == m:Seq.seq row {Seq.length m = 4})
-
-(* TODO: find a way not to duplicate the block spec *)
-inline_for_extraction noextract
-val mk_update_multi:
-  a : alg ->
-  m : valid_m_spec a ->
-  update_multi : blake2_update_multi_st a m ->
-  (i:G.erased index -> (
-  let i = G.reveal i in
-  s:s a m ->
-  prevlen:U64.t { U64.v prevlen % U32.v (block_len a) = 0 } ->
-  blocks:B.buffer uint8 { B.length blocks % U32.v (block_len a) = 0 } ->
-  len: U32.t { U32.v len = B.length blocks /\
-               U64.v prevlen + U32.v len <= max_input_length a } ->
-  ST.Stack unit
-  (requires fun h0 ->
-    let state = stateful_blake2 a m in
-    state.I.invariant #i h0 s /\
-    B.live h0 blocks /\
-    B.(loc_disjoint (state.I.footprint #i h0 s) (loc_buffer blocks)))
-  (ensures fun h0 _ h1 ->
-    let state = stateful_blake2 a m in
-    B.(modifies (state.I.footprint #i h0 s) h0 h1) /\
-    state.I.footprint #i h0 s == state.I.footprint #i h1 s /\
-    state.I.invariant #i h1 s /\
-    state.I.v i h1 s == update_multi_s #a i (state.I.v i h0 s) (U64.v prevlen)
-                                          (B.as_seq h0 blocks) /\
-    (state.I.freeable #i h0 s ==> state.I.freeable #i h1 s))))
-
-#push-options "--z3cliopt smt.arith.nl=false"
-let mk_update_multi a m update_multi i acc prevlen blocks len =
-  (**) size_block_props a;
-  [@inline_let] let wv = get_wv acc in
-  [@inline_let] let h = get_state_p acc in
-  (**) let h0 = ST.get () in
-  let nb = U32.(len /^ block_len a) in
-  (**) Math.Lemmas.div_exact_r (U32.v len) (U32.v (block_len a));
-  (**) Math.Lemmas.multiply_fractions (U32.v len) (U32.v (block_len a));
-  [@inline_let] let prevlen' = blake2_prevlen a prevlen in
-  (**) assert(Lib.Buffer.disjoint wv h);
-  update_multi #len wv h prevlen' blocks nb;
-  (**) let h3 = ST.get () in
-  (**) assert(s_v h3 acc ==
-  (**)    Loops.repeati #(Spec.Blake2.state a) (U32.v nb)
-  (**)                  (Spec.blake2_update1 a (Lib.IntTypes.uint_v prevlen')
-  (**)                                       (B.as_seq h0 blocks))
-  (**)                  (s_v h0 acc));
-  (**) state_types_equalities a;
-  (**) assert(Spec.Blake2.state a == Hash.words_state' (to_hash_alg a));
-  (**) update_multi_eq (U32.v nb) (s_v h0 acc) (U64.v prevlen) (B.as_seq h0 blocks);
-  (**) assert(Lib.IntTypes.uint_v prevlen' = U64.v prevlen);
-  (**) assert(s_v h3 acc == update_multi_s () (s_v h0 acc) (U64.v prevlen) (B.as_seq h0 blocks));
-  (**) assert(B.(modifies ((stateful_blake2 a m).I.footprint #() h0 acc) h0 h3))
-#pop-options
-
-inline_for_extraction noextract
-val mk_update_last:
-  a : alg ->
-  m : valid_m_spec a ->
-  update_last : blake2_update_last_st a m ->
-  (i: G.erased index -> (
-  let i = G.reveal i in
-  s:s a m ->
-  prevlen:U64.t { U64.v prevlen % U32.v (block_len a) = 0 } ->
-  last:B.buffer uint8 ->
-  last_len:U32.t{
-    last_len = B.len last /\
-    U32.v last_len <= U32.v (block_len a) /\
-    U64.v prevlen + U32.v last_len <= max_input_length a} ->
-  ST.Stack unit
-  (requires fun h0 ->
-    let state = stateful_blake2 a m in
-    state.I.invariant #i h0 s /\
-    B.live h0 last /\
-    B.(loc_disjoint (state.I.footprint #i h0 s) (loc_buffer last)))
-  (ensures fun h0 _ h1 ->
-    let state = stateful_blake2 a m in
-    state.I.invariant #i h1 s /\
-    state.I.v i h1 s == update_last_s #a i (state.I.v i h0 s)
-                                      (U64.v prevlen) (B.as_seq h0 last) /\
-    B.(modifies (state.I.footprint #i h0 s) h0 h1) /\
-    state.I.footprint #i h0 s == state.I.footprint #i h1 s /\
-    (state.I.freeable #i h0 s ==> state.I.freeable #i h1 s))))
-
-/// TODO: after analysis with quake, this proof sometimes loops
-#restart-solver
-#push-options "--ifuel 1 --z3cliopt smt.arith.nl=false"
-let mk_update_last a m update_last i acc prevlen last last_len =
-  (**) size_block_props a;
-  [@inline_let] let wv = get_wv acc in
-  [@inline_let] let h = get_state_p acc in
-  (**) let h0 = ST.get () in
-  (**) assert_norm(U64.v prevlen + U32.v last_len <= Spec.Blake2.max_limb a);
-  [@inline_let]
-  let prevlen' = blake2_prevlen a prevlen in
-  (**) assert((U64.v prevlen) % Hash.block_length (to_hash_alg a) = 0);
-  (**) assert(B.length last <= Hash.block_length (to_hash_alg a));
-  (**) assert(U64.v prevlen + B.length last <= max_input_length a);
-  update_last #last_len wv h prevlen' last_len last;
-  (* TODO: SH: if not put at the proper place, this call makes the proof loop or randomly fail *)
-  (**) update_last_eq (U64.v prevlen) (B.as_seq h0 last) (s_v h0 acc);
-  (**) let h2 = ST.get () in
-  (**) assert(
-  (**)   Core.state_v h2 h ==
-  (**)     Spec.blake2_update_last a (Lib.IntTypes.uint_v prevlen') (U32.v last_len)
-  (**)                               (B.as_seq h0 last)
-  (**)                               (Core.state_v h0 h));
-  (**) assert(s_v h2 acc ==
-  (**)   update_last_s () (s_v h0 acc) (U64.v prevlen) (B.as_seq h0 last))
-#pop-options
+/// Runtime
+/// -------
 
 let blocks_state_len (a : alg) (m : valid_m_spec a) :
   Tot (x:U32.t{
@@ -677,7 +401,7 @@ let blocks_state_len (a : alg) (m : valid_m_spec a) :
   | M128 -> block_len a
   | M256 -> block_len a
 
-#push-options "--ifuel 1 --z3cliopt smt.arith.nl=false"
+#push-options "--ifuel 1"// --z3cliopt smt.arith.nl=false"
 inline_for_extraction noextract
 let blake2 (a : alg) (m : valid_m_spec a)
            (init : blake2_init_st a m)
@@ -687,27 +411,27 @@ let blake2 (a : alg) (m : valid_m_spec a)
   I.block unit =
   I.Block
     I.Erased (* key management *)
-    
+
     (stateful_blake2 a m)     (* state *)
     (I.stateful_unused unit)  (* key *)
-    
+
     (fun () -> max_input_len a ) (* max_input_length *)
     (fun () -> output_len a) (* output_len *)
     (fun () -> block_len a) (* block_len *)
     (fun () -> blocks_state_len a m) (* blocks_state_len *)
-    
-    (fun () _k -> init_s a ()) (* init_s *)
-    (fun () acc prevlen input -> update_multi_s () acc prevlen input) (* update_multi_s *)
-    (fun () acc prevlen input -> update_last_s () acc prevlen input) (* update_last_s *)
-    (fun () _k acc -> finish_s #a () acc) (* finish_s *)
-    (fun () -> spec_s a ()) (* spec_s *)
+
+    (fun () _k -> init_s a) (* init_s *)
+    (fun () acc prevlen input -> update_multi_s acc prevlen input) (* update_multi_s *)
+    (fun () acc prevlen input -> update_last_s acc prevlen input) (* update_last_s *)
+    (fun () _k acc -> finish_s #a acc) (* finish_s *)
+    (fun () -> spec_s a) (* spec_s *)
 
     (* update_multi_zero *)
-    (fun () prevlen acc -> update_multi_zero () prevlen acc)
+    (fun () prevlen acc -> update_multi_zero prevlen acc)
     (* update_multi_associative *)
     (fun () acc prevlen1 prevlen2 input1 input2 ->
-      update_multi_associative () acc prevlen1 prevlen2 input1 input2)
-    (fun () _k input -> spec_is_incremental a () input) (* spec_is_incremental *)
+      update_multi_associative acc prevlen1 prevlen2 input1 input2)
+    (fun () _k input -> spec_is_incremental a input) (* spec_is_incremental *)
     (fun _ acc -> ()) (* index_of_state *)
 
     (* init *)
@@ -717,11 +441,15 @@ let blake2 (a : alg) (m : valid_m_spec a)
       init h (Lib.IntTypes.size 0) (output_len a))
 
     (* update_multi *)
-    (fun _ acc prevlen blocks len -> mk_update_multi a m update_multi () acc prevlen blocks len)
+    (fun _ acc prevlen blocks len ->
+      let wv, hash = acc in
+      let nb = len `U32.div` size_block a in
+      blake2_update_multi #a #m blake2_update_block #len wv hash (blake2_prevlen a prevlen) blocks nb)
 
     (* update_last *)
     (fun _ acc prevlen last last_len ->
-      mk_update_last a m update_last () acc prevlen last last_len)
+      let wv, hash = acc in
+      blake2_update_last #a #m blake2_update_block #last_len wv hash (blake2_prevlen a prevlen) last_len last)
 
     (* finish *)
     (fun _ k acc dst ->
